WIP:STORERA added in external call in SSAsm (left several trival lemmas)

x86/SSAsm.v
@@ -52,11 +52,13 @@ Inductive step  : state -> trace -> state -> Prop :=
                        (undef_regs (map preg_of (destroyed_by_builtin ef)) rs)) ->
       step (State rs m) t (State rs' m')
 | exec_step_external:
-    forall b ef args res rs m t rs' m',
+    forall b ef args res rs m t rs' m' m1,
       rs PC = Vptr b Ptrofs.zero ->
       Genv.find_funct_ptr ge b = Some (External ef) ->
-      extcall_arguments rs m (ef_sig ef) args ->
-      external_call ef ge args m t res m' ->
+      Mem.storev Mptr m (Val.offset_ptr (rs RSP) (Ptrofs.neg (Ptrofs.repr (size_chunk Mptr))))
+                 (rs RA) = Some m1 ->
+      extcall_arguments rs m1 (ef_sig ef) args ->
+      external_call ef ge args m1 t res m' ->
       rs' = (set_pair (loc_external_result (ef_sig ef)) res (undef_caller_save_regs rs)) #PC <- (rs RA) ->
       step (State rs m) t (State rs' m').
 
@@ -110,7 +112,7 @@ Ltac Equalities :=
   exploit external_call_determ. eexact H5. eexact H11. intros [A B].
   split. auto. intros. destruct B; auto. subst. auto.
 + assert (args0 = args) by (eapply extcall_arguments_determ; eauto). subst args0.
-  exploit external_call_determ. eexact H4. eexact H9. intros [A B].
+  exploit external_call_determ. eexact H5. eexact H11. intros [A B].
   split. auto. intros. destruct B; auto. subst. auto.
 - (* trace length *)
   red; intros; inv H; simpl.
