Makefile
@@ -112,8 +112,8 @@ BACKEND=\
   Mach.v \
   Bounds.v Stacklayout.v Stacking.v Stackingproof.v \
   Asm.v Asmgen.v Asmgenproof0.v Asmgenproof1.v Asmgenproof.v \
-  AsmFacts.v SSAsm.v SSAsmproof.v \
-  AsmRegs.v RealAsm.v RealAsmproof.v
+  AsmFacts.v AsmRegs.v SSAsm.v SSAsmproof.v \
+  RealAsm.v RealAsmproof.v
 
 # C front-end modules (in cfrontend/)
 
